theories/StackMachines/Reductions/PCTM_HALT_to_BSM_HALTING.v
@@ -1,0 +1,38 @@
+(**************************************************************)
+(*   Copyright Dominique Larchey-Wendling [*]                 *)
+(*                                                            *)
+(*                             [*] Affiliation LORIA -- CNRS  *)
+(**************************************************************)
+(*      This file is distributed under the terms of the       *)
+(*         CeCILL v2 FREE SOFTWARE LICENSE AGREEMENT          *)
+(**************************************************************)
+
+Require Import List Bool.
+
+From Undecidability.Synthetic
+  Require Import Undecidability ReducibilityFacts.
+
+From Undecidability.Shared.Libs.DLW 
+  Require Import pos vec sss compiler_correction.
+
+From Undecidability.TM
+  Require Import PCTM.
+
+From Undecidability.StackMachines.BSM 
+  Require Import bsm_defs bsm_pctm.
+
+Set Implicit Arguments.
+
+Set Default Proof Using "Type".
+
+Theorem PCTM_BSM_reduction : PCTM_HALT ⪯ BSM_HALTING.
+Proof.
+  apply reduces_dependent; exists.
+  intros (P,((l,b),r)).
+  set (Q := gc_code pctm_bsm2_compiler (1,P) 1).
+  set (w1 := l##(b::r)##vec_nil).
+  exists (existT _ 2 (existT _ 1 (existT _ Q w1))); simpl.
+  apply compiler_t_term_equiv; split; auto.
+Qed.
+
+Check PCTM_BSM_reduction.
