theories/TM/Reductions/SBTM_HALT_to_PCTM_HALT.v
@@ -1,0 +1,36 @@
+(**************************************************************)
+(*   Copyright Dominique Larchey-Wendling [*]                 *)
+(*                                                            *)
+(*                             [*] Affiliation LORIA -- CNRS  *)
+(**************************************************************)
+(*      This file is distributed under the terms of the       *)
+(*         CeCILL v2 FREE SOFTWARE LICENSE AGREEMENT          *)
+(**************************************************************)
+
+Require Import List Bool.
+
+From Undecidability.Synthetic
+  Require Import Undecidability ReducibilityFacts.
+
+From Undecidability.Shared.Libs.DLW 
+  Require Import pos sss.
+
+From Undecidability.TM 
+  Require Import SBTM PCTM pctm_sbtm.
+
+Set Implicit Arguments.
+
+Set Default Proof Using "Type".
+
+Theorem SBTM_PCTM_reduction : SBTM_HALT ⪯ PCTM_HALT.
+Proof.
+  apply reduces_dependent; exists.
+  intros (M,(i,t)).
+  exists (sbtm2pctm M i,t); split.
+  + intros (k & Hk).
+    apply sbtm2pctm_sound in Hk as (t' & Ht').
+    exists (0,t'); split; auto; left; auto.
+  + apply sbtm2pctm_complete.
+Qed.
+
+
